\documentclass[10pt,a4paper,fleqn]{article}
\usepackage[utf8]{inputenc}
\usepackage{amsmath}
\usepackage{amsfonts}
\usepackage{amssymb}
\title{"Basic DE's: Separation of Variables"}
\date{}
\begin{document}
  \maketitle 
  % This is a comment; it is not shown in the final output.
  % The following shows a little of the typesetting power of LaTeX
  \begin{align}
    dy/dx &= 2y + 1 \\
    \frac{dy}{2y+1} &= dx \\
    \int_a^b \frac{1}{2y+1}dy &= \int_a^b dx \\
  \end{align} 
    $u := 2y+1, f(u) := \frac{1}{2y+1}$
  \begin{align}
    \therefore \frac{dy}{du} \int_a^b \frac{1}{u} \frac{du}{dy} dy = \int \frac{1}{u} \frac{du}{dy} \frac{dy}{du}dy = \int \frac{1}{u}dy = \int_a^b \frac{1}{2y+1}dy &= \int_a^b dx \\
    \frac{dy}{du} \int_a^b \frac{1}{u} \frac{du}{dy} dy &= \int_a^b dx \\
  \end{align} 
$\because \int (f \circ g)g' = \int f$ \\
$\therefore \int f(g(y))g'(y)dy = \int f(u)u'dy = \int f(u) \frac{du}{dy}dy = \int f(u)du$ \\
  \begin{align} 
    \frac{dy}{du} \int_a^b \frac{1}{u} \frac{du}{dy} dy
                      &= \frac{dy}{du} \int_a^b f(u) du \\
                      &= \frac{dy}{du} \int_a^b \frac{1}{u} du \\
  \end{align}
%  
  \begin{align}
    \therefore \frac{dy}{du} \int_a^b \frac{1}{u} \frac{du}{dy} dy = \frac{dy}{du} \int_a^b \frac{1}{u} du &= \int_a^b dx \\
    \frac{dy}{du} \int_a^b \frac{1}{u} du &= \int_a^b dx
  \end{align}
$\because u = 2y+1 \therefore \frac{du}{dy} = 2$ \\
$\because \frac{dy}{du} = (\frac{du}{dy})^{-1} = 2^{-1} = \frac{1}{2}$ \\
  \begin{align}
    \frac{1}{2} \int_a^b \frac{1}{u} du = \frac{dy}{du} \int_a^b \frac{1}{u} du &= \int_a^b dx \\
    \frac{1}{2} \int_a^b \frac{1}{u} du &= \int_a^b dx \\
    \frac{1}{2} \ln|u| + c_1 &= x + c_2 \\
    \frac{1}{2} \ln|u| &= x + c_2 - c_1 \\
    \ln|u| &= 2 x + 2 (c_2 - c_1) \\
    \ln|u| &= 2 x + c_3 \\
    \ln|2y+1| &= 2 x + c_3 \because u = 2y+1 \\
    \because e^{\ln|2y+1|} &= e^{2 x + c_3} \\
    \therefore 2y+1 &= e^{2x}e^{c_3} \\
    2y &= e^{2x}e^{c_3} - 1 \\
    2y &= e^{2x}e^{c_3} - 1 \\
    2y &= C e^{2x} - 1 \\
    y  &= \frac{C e^{2x} - 1}{2} \ \ \ \blacksquare
  \end{align}
\end{document}
